\section{Features}

\frame{\sectionpage}

\begin{frame}[fragile]
  \frametitle{Functional}

  Programs are written like mathematical functions:

  \begin{semiverbatim}
f :: Int -> Int
f x = x + 1
  \end{semiverbatim}

  Datatypes are defined as alternatives:

  \begin{semiverbatim}
data IntList = Empty | Cons Int IntList
  \end{semiverbatim}
\end{frame}  

\begin{frame}[fragile]
  \frametitle{Functional}

  \begin{semiverbatim}
fib :: Int -> Int
fib n = loop 0 1 n
  where loop a b 0 = a
        loop a b i = loop b (a + b) (i - 1)
  \end{semiverbatim}

  versus
  
  \begin{semiverbatim}
int fib (int n) \{
    int a = 0, b = 1;
    for (int i = 0; i < n; ++i) \{
        int tmp = a;
        a = a + b;
        b = tmp;
    \}
    return a;
\}
  \end{semiverbatim}
\end{frame}

\begin{frame}[fragile]
  \frametitle{Lazy}

  Values aren't evaluated until needed

  Allows for infinite datastructues:

  \begin{semiverbatim}
takeWhile (\\x -> x < 100)
          (map (\\x -> x*x) [1..])
  \end{semiverbatim}
\end{frame}

\begin{frame}
  \frametitle{Type System}

  \begin{itemize}
  \item Type Inference
  \item Parametric Polymorphism
  \item Typeclasses
  \item ...And More!
  \end{itemize}
\end{frame} 

\begin{frame}[fragile]
  \frametitle{Type Inference}

  Statically typed, but don't need to write most types

  \begin{semiverbatim}
length [] = 0
length (x : xs) = 1 + length xs
  \end{semiverbatim}

  Type is inferred to be a list
\end{frame}

\begin{frame}[fragile]
  \frametitle{Parametric Polymorphism}

  Functions and data can work across many types:

  \begin{semiverbatim}
data List a = Nil | Cons a (List a)

append :: List a -> List a -> List a
  \end{semiverbatim}
\end{frame}

\begin{frame}
  \frametitle{Typeclasses}

  Like interfaces, but better type-safety

  \begin{semiverbatim}
(+) :: Num a => a -> a -> a
  \end{semiverbatim}
\end{frame}

\begin{frame}[fragile]
  \frametitle{Typeclasses}
  \begin{semiverbatim}
-- "Monoid" is fancy math speak for "Appendable"
concatTree :: Monoid a => Tree a -> a
concatTree (Leaf x) = x
concatTree (Branch left x right) =
  mconcat (concatTree left)
          (mconcat x (concatTree right))
  \end{semiverbatim}
\end{frame}

%% \begin{frame}
%%   \frametitle{And More}

  
